

Derivation of Expected Sample Variance for One Chain

Goal: Find $\mathbb{E} \left[\frac{1}{T-1} \sum_{t=1}^T (X_{m,t} - \bar{X}_m)^2 \right]$

Setup

- $X_{m,t}$ = sample t from chain m
- $\bar{X}_m = \frac{1}{T} \sum_{t=1}^T X_{m,t}$ = sample mean
- $\mu = \mathbb{E}[X_{m,t}]$ = true mean
- $\sigma^2 = \text{Var}(X_{m,t})$ = true variance

Step 1: Rewrite the deviation from sample mean

$$\sum_{t=1}^T (X_{m,t} - \bar{X}_m)^2 = \sum_{t=1}^T [(X_{m,t} - \mu) - (\bar{X}_m - \mu)]^2 \quad (1)$$

Step 2: Expand the square

$$= \sum_{t=1}^T [(X_{m,t} - \mu)^2 - 2(X_{m,t} - \mu)(\bar{X}_m - \mu) + (\bar{X}_m - \mu)^2] \quad (2)$$

$$= \sum_{t=1}^T (X_{m,t} - \mu)^2 - 2(\bar{X}_m - \mu) \sum_{t=1}^T (X_{m,t} - \mu) + T(\bar{X}_m - \mu)^2 \quad (3)$$

Step 3: Simplify the middle term

Note that:

$$\sum_{t=1}^T (X_{m,t} - \mu) = \sum_{t=1}^T X_{m,t} - T\mu \quad (4)$$

$$= T\bar{X}_m - T\mu \quad (5)$$

$$= T(\bar{X}_m - \mu) \quad (6)$$

Therefore:

$$\sum_{t=1}^T (X_{m,t} - \bar{X}_m)^2 = \sum_{t=1}^T (X_{m,t} - \mu)^2 - 2T(\bar{X}_m - \mu)^2 + T(\bar{X}_m - \mu)^2 \quad (7)$$

$$= \sum_{t=1}^T (X_{m,t} - \mu)^2 - T(\bar{X}_m - \mu)^2 \quad (8)$$

Step 4: Take expectations

$$\mathbb{E} \left[\sum_{t=1}^T (X_{m,t} - \bar{X}_m)^2 \right] = \mathbb{E} \left[\sum_{t=1}^T (X_{m,t} - \mu)^2 \right] - T \cdot \mathbb{E} [(\bar{X}_m - \mu)^2] \quad (9)$$

$$= \sum_{t=1}^T \mathbb{E} [(X_{m,t} - \mu)^2] - T \cdot \text{Var}(\bar{X}_m) \quad (10)$$

$$= T\sigma^2 - T \cdot \text{Var}(\bar{X}_m) \quad (11)$$

$$= T(\sigma^2 - \text{Var}(\bar{X}_m)) \quad (12)$$

Step 5: Divide by $(T - 1)$

$$\boxed{\mathbb{E} \left[\frac{1}{T-1} \sum_{t=1}^T (X_{m,t} - \bar{X}_m)^2 \right] = \frac{T}{T-1} (\sigma^2 - \text{Var}(\bar{X}_m))} \quad (13)$$

Key Insight

For i.i.d. samples: $\text{Var}(\bar{X}_m) = \sigma^2/T$, which gives:

$$\frac{T}{T-1} \left(\sigma^2 - \frac{\sigma^2}{T} \right) = \frac{T}{T-1} \cdot \frac{(T-1)\sigma^2}{T} = \sigma^2 \quad (14)$$

So the sample variance is unbiased.

For MCMC samples: Due to autocorrelation, $\text{Var}(\bar{X}_m) > \sigma^2/T$, which means:

$$\mathbb{E} \left[\frac{1}{T-1} \sum_{t=1}^T (X_{m,t} - \bar{X}_m)^2 \right] < \sigma^2 \quad (15)$$

Therefore, W **underestimates the true variance** σ^2 .

Derivation of $\mathbb{E}[B]$

Given:

$$B = \frac{1}{M-1} \sum_{m=1}^M (\bar{X}_m - \bar{X}_{..})^2 \quad (16)$$

where:

- $\bar{X}_m = \frac{1}{T} \sum_{t=1}^T X_{m,t}$ = mean of chain m
- $\bar{X}_{..} = \frac{1}{M} \sum_{m=1}^M \bar{X}_m$ = overall mean across all chains
- $\mu = \mathbb{E}[X_{m,t}]$ = true mean

Step 1: Rewrite deviations from overall mean

$$\sum_{m=1}^M (\bar{X}_m - \bar{X}_{..})^2 = \sum_{m=1}^M [(\bar{X}_m - \mu) - (\bar{X}_{..} - \mu)]^2 \quad (17)$$

Step 2: Expand the square

$$= \sum_{m=1}^M [(\bar{X}_m - \mu)^2 - 2(\bar{X}_m - \mu)(\bar{X}_{..} - \mu) + (\bar{X}_{..} - \mu)^2] \quad (18)$$

$$= \sum_{m=1}^M (\bar{X}_m - \mu)^2 - 2(\bar{X}_{..} - \mu) \sum_{m=1}^M (\bar{X}_m - \mu) + M(\bar{X}_{..} - \mu)^2 \quad (19)$$

Step 3: Simplify the middle term

Note that:

$$\sum_{m=1}^M (\bar{X}_m - \mu) = \sum_{m=1}^M \bar{X}_m - M\mu \quad (20)$$

$$= M\bar{X}_{..} - M\mu \quad (21)$$

$$= M(\bar{X}_{..} - \mu) \quad (22)$$

Therefore:

$$\sum_{m=1}^M (\bar{X}_m - \bar{X}_{..})^2 = \sum_{m=1}^M (\bar{X}_m - \mu)^2 - 2M(\bar{X}_{..} - \mu)^2 + M(\bar{X}_{..} - \mu)^2 \quad (23)$$

$$= \sum_{m=1}^M (\bar{X}_m - \mu)^2 - M(\bar{X}_{..} - \mu)^2 \quad (24)$$

Step 4: Take expectations

$$\mathbb{E} \left[\sum_{m=1}^M (\bar{X}_m - \bar{X}_{..})^2 \right] = \mathbb{E} \left[\sum_{m=1}^M (\bar{X}_m - \mu)^2 \right] - M \cdot \mathbb{E} [(\bar{X}_{..} - \mu)^2] \quad (25)$$

$$= \sum_{m=1}^M \mathbb{E} [(\bar{X}_m - \mu)^2] - M \cdot \mathbb{E} [(\bar{X}_{..} - \mu)^2] \quad (26)$$

$$= M \cdot \text{Var}(\bar{X}_m) - M \cdot \text{Var}(\bar{X}_{..}) \quad (27)$$

(assuming all chains have the same variance of their means)

Step 5: Find $\text{Var}(\bar{X}_{..})$

Since $\bar{X}_{..} = \frac{1}{M} \sum_{m=1}^M \bar{X}_m$ and assuming chains are independent:

$$\text{Var}(\bar{X}_{..}) = \text{Var}\left(\frac{1}{M} \sum_{m=1}^M \bar{X}_m\right) \quad (28)$$

$$= \frac{1}{M^2} \sum_{m=1}^M \text{Var}(\bar{X}_m) \quad (29)$$

$$= \frac{1}{M^2} \cdot M \cdot \text{Var}(\bar{X}_m) \quad (30)$$

$$= \frac{1}{M} \text{Var}(\bar{X}_m) \quad (31)$$

Step 6: Substitute back

$$\mathbb{E}\left[\sum_{m=1}^M (\bar{X}_m - \bar{X}_{..})^2\right] = M \cdot \text{Var}(\bar{X}_m) - M \cdot \frac{1}{M} \text{Var}(\bar{X}_m) \quad (32)$$

$$= M \cdot \text{Var}(\bar{X}_m) - \text{Var}(\bar{X}_m) \quad (33)$$

$$= (M - 1) \text{Var}(\bar{X}_m) \quad (34)$$

Step 7: Divide by $(M - 1)$

$$\boxed{\mathbb{E}[B] = \frac{1}{M - 1} \cdot (M - 1) \text{Var}(\bar{X}_m) = \text{Var}(\bar{X}_m)} \quad (35)$$

Conclusion

This confirms what's stated on slide 6: $\mathbb{E}[B] = \text{Var}(\bar{X}_m)$

The between-chain variance B is an unbiased estimator of the variance of the chain means!

Derivation of the Gelman-Rubin Variance Estimator

The derivation follows these steps:

1. **Equation (2)** shows that the sample variance s_i^2 is biased for the target variance σ^2 :

$$E_F[s_i^2] = \frac{n}{n - 1} (\sigma^2 - \text{Var}_F(\bar{X}_{i.})) \quad (36)$$

2. **Key insight:** For correlated MCMC samples, $\text{Var}_F(\bar{X}_{i.})$ is much larger than σ^2/n (which would be the case for independent samples). This means s_i^2 systematically underestimates σ^2 .
3. **Rearranging equation (2)** to solve for σ^2 :

$$\sigma^2 = \frac{n-1}{n} E_F[s_i^2] + \text{Var}_F(\bar{X}_{i.}) \quad (37)$$

4. **Equation (3)** provides an estimator for $\text{Var}_F(\bar{X}_{i.})$:

$$\frac{B}{n} = \frac{1}{m-1} \sum_{i=1}^m (\bar{X}_{i.} - \hat{\mu})^2 \quad (38)$$

This is the sample variance of the m chain means, which estimates the variance of $\bar{X}_{i.}$.

5. **Final estimator:** Substituting the sample quantities:
 - Use s^2 (the average of the m sample variances) to estimate $E_F[s_i^2]$
 - Use B/n to estimate $\text{Var}_F(\bar{X}_{i.})$

This gives:

$$\boxed{\hat{\sigma}^2 = \frac{n-1}{n} s^2 + \frac{B}{n}} \quad (39)$$

Intuition: Gelman-Rubin corrects for the downward bias in s^2 by adding back an estimate of the between-chain variance (B/n), which captures the additional variability due to correlation in the Markov chains.